src/lowparse/LowParse.Low.Option.fst
@@ -4,6 +4,8 @@ include LowParse.Low.Base
 
 module HST = FStar.HyperStack.ST
 module U32 = FStar.UInt32
+module U64 = FStar.UInt64
+module Cast = FStar.Int.Cast
 
 inline_for_extraction
 let validate_option (#k: parser_kind) (#t: Type) (#p: parser k t) (v: validator p) : Tot (validator (parse_option p)) =
@@ -12,6 +14,6 @@ let validate_option (#k: parser_kind) (#t: Type) (#p: parser k t) (v: validator 
   [@inline_let] let _ = valid_facts (parse_option p) h input pos in
   [@inline_let] let _ = valid_facts p h input pos in
   let r = v input pos in
-  if validator_max_length `U32.lt` r
-  then pos
+  if validator_max_length `U64.lt` r
+  then Cast.uint32_to_uint64 pos
   else r
